template-coq/theories/utils/MCString.v
@@ -1,11 +1,12 @@
-From Coq Require Import String Decimal DecimalString ZArith.
-From MetaCoq.Template Require Import MCCompare.
+From Coq Require Import Decimal DecimalString ZArith.
+From MetaCoq.Template Require Import MCCompare bytestring.
 
-Local Open Scope string_scope.
+Local Open Scope bs.
+Notation string := String.t.
 
 (** When defining [Show] instance for your own datatypes, you sometimes need to
     start a new line for better printing. [nl] is a shorthand for it. *)
-Definition nl : string := String (Ascii.ascii_of_nat 10) EmptyString.
+Definition nl : string := String.String "010"%byte String.EmptyString.
 
 Definition string_of_list_aux {A} (f : A -> string) (sep : string) (l : list A) : string :=
   let fix aux l :=
@@ -26,7 +27,7 @@ Definition parens (top : bool) (s : string) :=
   if top then s else "(" ++ s ++ ")".
 
 Definition string_of_nat n : string :=
-  DecimalString.NilEmpty.string_of_uint (Nat.to_uint n).
+  String.of_string (DecimalString.NilEmpty.string_of_uint (Nat.to_uint n)).
 
 #[global]
 Hint Resolve String.string_dec : eq_dec.
@@ -41,14 +42,10 @@ Definition string_of_Z (z : Z) : string :=
   | Zneg p => "-" ++ string_of_positive p
   end.
 
-Definition eq_string s s' :=
-  match string_compare s s' with
-  | Eq => true
-  | _ => false
-  end.
+Definition eq_string := StringOT.eqb.
 
 Lemma eq_string_refl x : is_true (eq_string x x).
 Proof.
-  unfold eq_string.
-  now rewrite (proj2 (string_compare_eq x x) eq_refl).
+  unfold eq_string, StringOT.eqb.
+  now rewrite StringOT.compare_refl.
 Qed.
