template-coq/theories/utils/ByteCompareSpec.v
@@ -1,0 +1,92 @@
+From Coq Require Import Byte.
+From MetaCoq.Template Require Import Reflect ByteCompare.
+From Equations Require Import Equations.
+
+Ltac solve_noconf ::= idtac.
+Derive NoConfusion for byte.
+Next Obligation.
+  destruct a; abstract (destruct b; try exact (False_ind _ H); exact eq_refl).
+Defined.
+Next Obligation.
+  destruct b; cbn; exact I.
+Defined.
+Next Obligation.
+  destruct a; abstract (destruct b; try (exact (False_ind _ e)); destruct e; exact eq_refl).
+Defined.
+Next Obligation.
+  destruct b; cbn; exact eq_refl.
+Defined.
+
+Lemma reflect_equiv P Q b : P <-> Q -> Bool.reflect P b -> Bool.reflect Q b.
+Proof.
+  intros eq r. destruct r.
+  - now constructor; apply eq.
+  - constructor. now rewrite <- eq.
+Qed.
+
+Program Instance eqb_spec : ReflectEq byte := 
+  {| Reflect.eqb := eqb |}.
+Next Obligation.
+  apply (reflect_equiv (NoConfusion x y)).
+  split; intros. now apply noConfusion. now apply noConfusion_inv.
+  destruct x; cbn; abstract (destruct y; cbn; constructor; try exact (fun f => f); exact I).
+Qed.
+
+Definition lt x y := compare x y = Lt.
+
+Require Import MCCompare.
+
+Lemma compare_opp x y : compare x y = CompOpp (compare y x).
+Proof.
+  destruct x; abstract (destruct y; exact eq_refl).
+Qed.
+
+Lemma compare_eq x y : compare x y = Eq -> x = y.
+Proof.
+  intros. eapply noConfusion.
+  destruct x; abstract (apply noConfusion_inv in H; destruct y; exact H).
+Qed.
+
+Lemma compare_spec x y : CompareSpec (x = y) (lt x y) (lt y x) (compare x y).
+Proof.
+  destruct (compare x y) eqn:comp.
+  - constructor. now apply compare_eq in comp.
+  - constructor. exact comp.
+  - constructor. red. now rewrite compare_opp, comp.
+Qed.
+
+Lemma compare_equiv x y : compare x y = Nat.compare (Strings.Byte.to_nat x) (Strings.Byte.to_nat y).
+Proof.
+  destruct x; abstract (destruct y; exact eq_refl).
+Qed.
+
+From Coq Require Import Lia.
+
+Lemma lt_trans x y z : lt x y -> lt y z -> lt x z.
+Proof.
+  unfold lt.
+  rewrite !compare_equiv.
+  rewrite <- !Compare_dec.nat_compare_lt. lia.
+Qed.
+
+Lemma lt_not_eq x y : lt x y -> x <> y.
+Proof.
+  unfold lt.
+  rewrite !compare_equiv.
+  rewrite <- !Compare_dec.nat_compare_lt. intros Hlt Heq. subst. lia.
+Qed.
+
+Lemma compare_eq' x y : compare x y = Eq -> x = y.
+Proof.
+  rewrite compare_equiv.
+  intros Hcomp.
+  eapply PeanoNat.Nat.compare_eq in Hcomp.
+  eapply (f_equal of_nat) in Hcomp.
+  rewrite !of_to_nat in Hcomp. now noconf Hcomp.
+Qed.
+
+Lemma compare_eq_refl x : compare x x = Eq.
+Proof.
+  rewrite compare_equiv.
+  eapply PeanoNat.Nat.compare_refl.
+Qed.
