template-coq/theories/utils/bytestring.v
@@ -1,0 +1,378 @@
+(**
+ * Copyright (C) 2020 BedRock Systems, Inc.
+ * All rights reserved.
+ *
+ * SPDX-License-Identifier: LGPL-2.1 WITH BedRock Exception for use over network,
+ * see repository root for details.
+ *)
+ 
+Require Coq.Strings.String.
+Require Import Coq.NArith.NArith.
+Require Import Coq.micromega.Lia.
+From Equations Require Import Equations. 
+Set Primitive Projections.
+Set Default Proof Using "Type".
+
+(** bytes *)
+
+Definition byte_parse (b : Byte.byte) : Byte.byte := b.
+Definition byte_print (b : Byte.byte) : Byte.byte := b.
+
+Delimit Scope byte_scope with byte.
+String Notation Byte.byte byte_parse byte_print : byte_scope.
+
+Bind Scope byte_scope with Byte.byte.
+
+Definition byte_cmp (a b : Byte.byte) : comparison :=
+  N.compare (Byte.to_N a) (Byte.to_N b).
+ 
+Declare Scope bs_scope.
+Delimit Scope bs_scope with bs.
+
+(** bytestrings *)
+Module String.
+  Inductive t : Set :=
+  | EmptyString
+  | String (_ : Byte.byte) (_ : t).
+  Bind Scope bs_scope with t.
+
+  Fixpoint print (b : t) : list Byte.byte :=
+    match b with
+    | EmptyString => nil
+    | String b bs => b :: print bs
+    end.
+
+  Fixpoint parse (b : list Byte.byte) : t :=
+    match b with
+    | nil => EmptyString
+    | List.cons b bs => String b (parse bs)
+    end.
+
+  Lemma print_parse_inv:
+    forall x : t, parse (print x) = x.
+  Proof.
+    induction x; simpl; intros; auto.
+    f_equal; auto.
+  Qed.
+
+  Fixpoint append (x y : t) : t :=
+    match x with
+    | EmptyString => y
+    | String x xs => String x (append xs y)
+    end.
+  
+  Notation "x ++ y" := (append x y) : bs_scope.
+  
+  Fixpoint to_string (b : t) : String.string :=
+    match b with
+    | EmptyString => Strings.String.EmptyString
+    | String x xs => Strings.String.String (Ascii.ascii_of_byte x) (to_string xs)
+    end.
+  
+  Fixpoint of_string (b : String.string) : t :=
+    match b with
+    | Strings.String.EmptyString => EmptyString
+    | Strings.String.String x xs => String (Ascii.byte_of_ascii x) (of_string xs)
+    end%bs.
+  
+  Fixpoint rev (acc s : t) : t :=
+    match s with
+    | EmptyString => acc
+    | String s ss => rev (String s acc) ss
+    end.
+    
+  (** *** Substrings *)
+
+  (** [substring n m s] returns the substring of [s] that starts
+      at position [n] and of length [m];
+      if this does not make sense it returns [""] *)
+  
+  Fixpoint substring (n m : nat) (s : t) : t :=
+    match n, m, s with
+    | O, O, _ => EmptyString
+    | O, S m', EmptyString => s
+    | O, S m', String c s' => String c (substring 0 m' s')
+    | S n', _, EmptyString => s
+    | S n', _, String c s' => substring n' m s'
+    end.
+  
+  Fixpoint prefix (s1 s2 : t) {struct s1} : bool :=
+    match s1 with
+    | EmptyString => true
+    | String x xs =>
+      match s2 with
+      | EmptyString => false
+      | String y ys =>
+        if Byte.eqb x y then prefix xs ys
+        else false
+      end
+    end%bs.
+  
+  Fixpoint index (n : nat) (s1 s2 : t) {struct s2} : option nat :=
+    match s2 with
+    | EmptyString =>
+        match n with
+        | 0 => match s1 with
+              | EmptyString => Some 0
+              | String _ _ => None
+              end
+        | S _ => None
+        end
+    | String _ s2' =>
+        match n with
+        | 0 =>
+            if prefix s1 s2
+            then Some 0
+            else match index 0 s1 s2' with
+                | Some n0 => Some (S n0)
+                | None => None
+                end
+        | S n' => match index n' s1 s2' with
+                  | Some n0 => Some (S n0)
+                  | None => None
+                  end
+        end
+    end%bs.
+  
+  Fixpoint length (l : t) : nat :=
+    match l with
+    | EmptyString => 0
+    | String _ l => S (length l)
+    end.
+  
+  Local Fixpoint contains (start: nat) (keys: list t) (fullname: t) :bool :=
+    match keys with
+    | List.cons kh ktl =>
+      match index start kh fullname with
+      | Some n => contains (n + length kh) ktl fullname
+      | None => false
+      end
+    | List.nil => true
+    end.
+  
+  Fixpoint eqb (a b : t) : bool :=
+    match a , b with
+    | EmptyString , EmptyString => true
+    | String x xs , String y ys =>
+      if Byte.eqb x y then eqb xs ys else false
+    | _ , _ => false
+    end.
+  
+  Fixpoint concat (sep : t) (s : list t) : t :=
+    match s with
+    | nil => EmptyString
+    | cons s xs => s ++ sep ++ concat sep xs
+    end.
+
+End String.
+
+Definition bs := String.t.
+ 
+Bind Scope bs_scope with bs.
+
+String Notation String.t String.parse String.print : bs_scope.
+
+Notation "x ++ y" := (String.append x y) : bs_scope.
+  
+Import String.
+
+(** comparison *)
+Require Import Coq.Structures.OrderedType.
+
+Lemma to_N_inj : forall x y, Byte.to_N x = Byte.to_N y <-> x = y.
+Proof.
+  split.
+  2: destruct 1; reflexivity.
+  intros.
+  assert (Some x = Some y).
+  { do 2 rewrite <- Byte.of_to_N.
+    destruct H. reflexivity. }
+  injection H0. auto.
+Qed.
+
+Module OT_byte <: OrderedType.OrderedType with Definition t := Byte.byte.
+  Definition t := Byte.byte.
+  Definition eq := fun l r => byte_cmp l r = Eq.
+  Definition lt := fun l r => byte_cmp l r = Lt.
+  Theorem eq_refl : forall x : t, eq x x.
+  Proof.
+    intros; apply N.compare_refl.
+  Qed.
+  Theorem eq_sym : forall x y : t, eq x y -> eq y x.
+  Proof.
+    intros. eapply N.compare_eq in H. red. unfold byte_cmp.
+    destruct H. apply eq_refl.
+  Qed.
+  Theorem eq_trans : forall x y z : t, eq x y -> eq y z -> eq x z.
+  Proof.
+    intros. eapply N.compare_eq in H. eapply N.compare_eq in H0.
+    red. unfold byte_cmp.
+    destruct H. destruct H0. apply eq_refl.
+  Qed.
+  Theorem lt_trans : forall x y z : t, lt x y -> lt y z -> lt x z.
+  Proof.
+    unfold lt, byte_cmp.
+    intros.
+    rewrite N.compare_lt_iff in H.
+    rewrite N.compare_lt_iff in H0.
+    rewrite N.compare_lt_iff.
+    etransitivity; eassumption.
+  Qed.
+  Theorem lt_not_eq : forall x y : t, lt x y -> not (eq x y).
+  Proof.
+    unfold lt, eq, byte_cmp; intros.
+    rewrite N.compare_lt_iff in H.
+    rewrite N.compare_eq_iff.
+    lia.
+  Qed.
+  Definition compare (x y : t) : OrderedType.Compare lt eq x y.
+    refine  (
+    match byte_cmp x y as X return byte_cmp x y = X -> OrderedType.Compare lt eq x y  with
+    | Eq => fun pf => OrderedType.EQ pf
+    | Lt => fun pf => OrderedType.LT pf
+    | Gt => fun pf => OrderedType.GT _
+    end (Logic.eq_refl)).
+    unfold lt, byte_cmp.
+    rewrite N.compare_antisym.
+    apply CompOpp_iff. apply pf.
+  Defined.
+
+  Definition eq_dec : forall x y : t, {eq x y} + {not (eq x y)}.
+  refine (fun x y =>
+      match byte_cmp x y as Z return byte_cmp x y = Z -> _ with
+      | Eq => fun pf => left pf
+      | _ => fun _ => right _
+      end Logic.eq_refl).
+  unfold eq. congruence.
+  unfold eq. congruence.
+  Defined.
+
+End OT_byte.
+
+Fixpoint bs_cmp (xs ys : bs) : comparison :=
+  match xs , ys with
+  | EmptyString , EmptyString => Eq
+  | EmptyString , _ => Lt
+  | _ , EmptyString => Gt
+  | String x xs , String y ys =>
+    match byte_cmp x y with
+    | Eq => bs_cmp xs ys
+    | x => x
+    end
+  end%bs.
+
+Lemma byte_cmp_refl : forall a, byte_cmp a a = Eq.
+Proof.
+  intros. unfold byte_cmp.
+  eapply N.compare_refl.
+Defined.
+
+Theorem byte_cmp_spec : forall x y, CompareSpec (x = y) (OT_byte.lt x y) (OT_byte.lt y x) (byte_cmp x y).
+Proof.
+  intros. unfold byte_cmp.
+  unfold OT_byte.lt, byte_cmp.
+  destruct (N.compare_spec (Byte.to_N x) (Byte.to_N y)); constructor; auto.
+  apply to_N_inj. assumption.
+Qed.
+
+Lemma byte_cmp_eq : forall x y, byte_cmp x y = Eq <-> x = y.
+Proof.
+  intros. destruct (byte_cmp_spec x y); split; intros; subst; try congruence.
+  eapply OT_byte.lt_not_eq in H. elim H; eapply byte_cmp_refl.
+  eapply OT_byte.lt_not_eq in H. elim H; eapply byte_cmp_refl.
+Defined.
+
+Global Instance byte_eqdec : Classes.EqDec Byte.byte.
+Proof. intros x y.
+  destruct (OT_byte.eq_dec x y).
+  now left; eapply byte_cmp_eq in e.
+  right. intros H; subst y. apply n. apply byte_cmp_refl.
+Qed.
+
+Module OT_bs <: OrderedType.OrderedType with Definition t := bs.
+  Definition t := bs.
+  Definition eq := @eq bs.
+  Definition lt := fun l r => bs_cmp l r = Lt.
+
+  Theorem lm : forall x y, CompareSpec (x = y) (lt x y) (lt y x) (bs_cmp x y).
+  Proof.
+    induction x; destruct y; simpl.
+    - constructor; reflexivity.
+    - constructor. reflexivity.
+    - constructor. reflexivity.
+    - unfold lt; simpl.
+      destruct (byte_cmp_spec b b0); simpl.
+      + subst. destruct (IHx y); constructor; eauto.
+        congruence.
+        destruct (byte_cmp_spec b0 b0); try congruence.
+        red in H0. rewrite OT_byte.eq_refl in H0. congruence.
+      + constructor; auto.
+      + red in H. rewrite H. constructor; auto.
+  Qed.
+
+  Definition compare (x y : t) : OrderedType.Compare lt eq x y.
+    refine  (
+    match bs_cmp x y as X return bs_cmp x y = X -> OrderedType.Compare lt eq x y  with
+    | Eq => fun pf => OrderedType.EQ _
+    | Lt => fun pf => OrderedType.LT pf
+    | Gt => fun pf => OrderedType.GT _
+    end (Logic.eq_refl)).
+    generalize (lm x y). rewrite pf. inversion 1; auto.
+    generalize (lm x y). rewrite pf. inversion 1; auto.
+  Defined.
+
+  Theorem eq_refl : forall x : t, eq x x.
+  Proof.
+    reflexivity.
+  Qed.
+  Theorem eq_sym : forall x y : t, eq x y -> eq y x.
+  Proof.
+    eapply eq_sym.
+  Qed.
+  Theorem eq_trans : forall x y z : t, eq x y -> eq y z -> eq x z.
+  Proof.
+    eapply eq_trans.
+  Qed.
+  Theorem lt_trans : forall x y z : t, lt x y -> lt y z -> lt x z.
+  Proof.
+    unfold lt.
+    induction x; destruct y; simpl; try congruence.
+    - destruct z; congruence.
+    - destruct (byte_cmp_spec b b0); subst.
+      + destruct z; auto.
+        destruct (byte_cmp b0 b); auto.
+        eauto.
+      + destruct z; auto.
+        red in H.
+        destruct (byte_cmp b0 b1) eqn:?.
+        * generalize (byte_cmp_spec b0 b1).
+          rewrite Heqc. inversion 1.
+          subst. rewrite H. auto.
+        * generalize (OT_byte.lt_trans _ _ _ H Heqc). unfold OT_byte.lt.
+          intro X; rewrite X. auto.
+        * congruence.
+      + congruence.
+  Qed.
+  Theorem lt_not_eq : forall x y : t, lt x y -> not (eq x y).
+  Proof.
+    unfold lt, eq.
+    intros. intro. subst.
+    induction y; simpl in *; try congruence.
+    rewrite byte_cmp_refl in *. auto.
+  Qed.
+
+  Definition eq_dec : forall x y : t, {eq x y} + {not (eq x y)}.
+    refine (fun x y =>
+        match bs_cmp x y as Z return CompareSpec _ _ _ Z -> _ with
+        | Eq => fun pf => left _
+        | _ => fun _ => right _
+        end (lm x y)).
+    - inversion pf. apply H.
+    - apply lt_not_eq. inversion c. auto.
+    - inversion c. apply lt_not_eq in H.
+      unfold eq in *. congruence.
+  Defined.
+
+End OT_bs.
+
+Global Instance string_eq_dec : EqDec bs := { eq_dec := OT_bs.eq_dec }.
