test-suite/bugkncst.v
@@ -13,8 +13,6 @@ Function Plus1 (n: nat) {measure id n} : nat :=
 Defined.
 
 Require Import Coq.Lists.List.
-Require Import Coq.Strings.String.
-Require Import Coq.Strings.Ascii.
 Require Import Coq.Bool.Bool.
 Require Import MetaCoq.Template.Loader.
 Require Import MetaCoq.Template.All.
@@ -55,7 +53,7 @@ Fixpoint pocc_term (n:nat) (t:term): bool :=
   (** does [tConst str] occur anywhere in a program? **)
 
 Definition bound_global_decl (d : kername * global_decl) : bool :=
-  if kername_eq_dec str (fst d) then true else false.
+  if eq_kername str (fst d) then true else false.
 
 Definition bound_program (p : program) := List.existsb bound_global_decl (fst p).(declarations).
 
@@ -70,7 +68,7 @@ Definition pocc_program p := pocc_term 2000 (snd p) || List.existsb pocc_global_
 
 End occ_term_Sec.
 
-Require Import List String. Import ListNotations. Open Scope string_scope.
+Require Import List. Import ListNotations. Open Scope bs_scope.
 (* MetaCoq Test Unquote (tConst (MPfile ["Nat"; "PeanoNat"; "Arith"; "Coq"], "pred") []) . *)
 
 Eval vm_compute in (eq_refl : pocc_program (MPfile ["Nat"; "PeanoNat"; "Arith"; "Coq"], "pred") p_Plus1 = false).
